src/DY.Lib.Event.Typed.fst
@@ -1,0 +1,189 @@
+module DY.Lib.Event.Typed
+
+open Comparse
+open DY.Core
+open DY.Lib.SplitPredicate
+open DY.Lib.Comparse.Glue
+
+(*** Event typeclass ***)
+
+class event (a:Type0) = {
+  tag: string;
+  [@@@FStar.Tactics.Typeclasses.tcinstance]
+  format: parseable_serializeable bytes a;
+}
+
+val mk_event_instance:
+  #a:Type0 -> {|parseable_serializeable bytes a|} -> string ->
+  event a
+let mk_event_instance #a #format tag = {
+  tag;
+  format;
+}
+
+(*** Split predicate ***)
+
+type event_predicate (a:Type0) {|event a|} =
+  trace -> principal -> a -> prop
+
+let split_event_pred_func: split_predicate_input_values = {
+  labeled_data_t = trace & principal & string & bytes;
+  label_t = string;
+  encoded_label_t = string;
+  raw_data_t = trace & principal & bytes;
+
+  decode_labeled_data = (fun (tr, prin, tag, content) -> (
+    Some (tag, (tr, prin, content))
+  ));
+
+  encode_label = (fun s -> s);
+  encode_label_inj = (fun l1 l2 -> ());
+
+  local_pred = trace -> principal -> bytes -> prop;
+  global_pred = trace -> principal -> string -> bytes -> prop;
+
+  apply_local_pred = (fun epred (tr, prin, content) ->
+    epred tr prin content
+  );
+  apply_global_pred = (fun epred (tr, prin, tag, content) ->
+    epred tr prin tag content
+  );
+  mk_global_pred = (fun spred -> fun tr prin tag content ->
+    spred (tr, prin, tag, content)
+  );
+  apply_mk_global_pred = (fun spred x -> ());
+}
+
+type compiled_event_predicate = split_event_pred_func.local_pred
+
+val compile_event_pred:
+  #a:Type0 -> {|event a|} ->
+  event_predicate a ->
+  compiled_event_predicate
+let compile_event_pred #a #ev epred tr prin content_bytes =
+  match parse a content_bytes with
+  | None -> False
+  | Some(content) -> epred tr prin content
+
+val has_compiled_event_pred:
+  protocol_invariants -> (string & compiled_event_predicate) -> prop
+let has_compiled_event_pred invs (label, epred) =
+  has_local_pred split_event_pred_func event_pred (label, epred)
+
+val has_event_pred:
+  #a:Type0 -> {|event a|} ->
+  protocol_invariants -> event_predicate a -> prop
+let has_event_pred #a #ev invs epred =
+  has_compiled_event_pred invs (ev.tag, compile_event_pred epred)
+
+(*** Global event predicate builder ***)
+
+val mk_event_pred: {|crypto_invariants|} -> list (string & compiled_event_predicate) -> trace -> principal -> string -> bytes -> prop
+let mk_event_pred #cinvs l =
+  mk_global_pred split_event_pred_func l
+
+val mk_event_pred_correct: invs:protocol_invariants -> lpreds:list (string & compiled_event_predicate) -> Lemma
+  (requires
+    invs.trace_invs.event_pred == mk_event_pred lpreds /\
+    List.Tot.no_repeats_p (List.Tot.map fst lpreds)
+  )
+  (ensures for_allP (has_compiled_event_pred invs) lpreds)
+let mk_event_pred_correct invs lpreds =
+  for_allP_eq (has_compiled_event_pred invs) lpreds;
+  FStar.Classical.forall_intro_2 (FStar.Classical.move_requires_2 (mk_global_pred_correct split_event_pred_func lpreds))
+
+(*** Monadic functions ***)
+
+[@@ "opaque_to_smt"]
+val trigger_event:
+  #a:Type -> {|event a|} ->
+  principal -> a ->
+  crypto unit
+let trigger_event #a #ev prin e =
+  DY.Core.trigger_event prin ev.tag (serialize a e)
+
+[@@ "opaque_to_smt"]
+val event_triggered_at:
+  #a:Type -> {|event a|} ->
+  trace -> nat -> principal -> a ->
+  prop
+let event_triggered_at #a #ev tr i prin e =
+  DY.Core.event_triggered_at tr i prin ev.tag (serialize a e)
+
+val event_triggered:
+  #a:Type -> {|event a|} ->
+  trace -> principal -> a ->
+  prop
+let event_triggered #a #ev tr prin e =
+  exists i. event_triggered_at tr i prin e
+
+val trigger_event_trace_invariant:
+  {|invs:protocol_invariants|} ->
+  #a:Type -> {|ev:event a|} ->
+  epred:event_predicate a ->
+  prin:principal -> e:a -> tr:trace ->
+  Lemma
+  (requires
+    epred tr prin e /\
+    has_event_pred invs epred /\
+    trace_invariant tr
+  )
+  (ensures (
+    let ((), tr_out) = trigger_event prin e tr in
+    trace_invariant tr_out /\
+    event_triggered tr_out prin e
+  ))
+  [SMTPat (trigger_event prin e tr);
+   SMTPat (has_event_pred invs epred);
+   SMTPat (trace_invariant tr)]
+let trigger_event_trace_invariant #invs #a #ev epred prin e tr =
+  reveal_opaque (`%trigger_event) (trigger_event #a);
+  reveal_opaque (`%event_triggered_at) (event_triggered_at #a);
+  local_eq_global_lemma split_event_pred_func event_pred ev.tag (compile_event_pred epred) (tr, prin, ev.tag, serialize _ e) (tr, prin, serialize _ e)
+
+val event_triggered_at_implies_pred:
+  {|invs:protocol_invariants|} ->
+  #a:Type -> {|ev:event a|} ->
+  epred:event_predicate a -> tr:trace ->
+  i:nat -> prin:principal -> e:a ->
+  Lemma
+  (requires
+    event_triggered_at tr i prin e /\
+    has_event_pred invs epred /\
+    trace_invariant tr
+  )
+  (ensures i <= DY.Core.Trace.Type.length tr /\ epred (prefix tr i) prin e)
+  [SMTPat (event_triggered_at tr i prin e);
+   SMTPat (has_event_pred invs epred);
+   SMTPat (trace_invariant tr);
+  ]
+let event_triggered_at_implies_pred #invs #a #ev epred tr i prin e =
+  reveal_opaque (`%event_triggered_at) (event_triggered_at #a);
+  local_eq_global_lemma split_event_pred_func event_pred ev.tag (compile_event_pred epred) ((prefix tr i), prin, ev.tag, serialize _ e) ((prefix tr i), prin, serialize _ e)
+
+val event_triggered_grows:
+  #a:Type -> {|ev:event a|} ->
+  tr1:trace -> tr2:trace ->
+  prin:principal -> e:a  ->
+  Lemma
+  (requires event_triggered tr1 prin e /\ tr1 <$ tr2)
+  (ensures event_triggered tr2 prin e)
+  [SMTPat (event_triggered tr1 prin e); SMTPat (tr1 <$ tr2)]
+let event_triggered_grows #a #ev tr1 tr2 prin e =
+  reveal_opaque (`%event_triggered_at) (event_triggered_at #a);
+  ()
+
+val event_triggered_at_implies_trace_event_at:
+  #a:Type -> {|ev:event a|} ->
+  tr:trace -> i:nat -> prin:principal -> e:a  ->
+  Lemma
+  (requires event_triggered_at tr i prin e)
+  (ensures
+    i < DY.Core.Trace.Type.length tr /\
+    get_event_at tr i == Event prin ev.tag (serialize a e) /\
+    parse #bytes a (serialize a e) == Some e
+  )
+  [SMTPat (event_triggered_at tr i prin e)]
+let event_triggered_at_implies_trace_event_at #a #ev tr i prin e =
+  reveal_opaque (`%event_triggered_at) (event_triggered_at #a);
+  ()
